Shuffled files in preparation for typechecking step

02Typed/Typed.thy
@@ -1,79 +1,79 @@
-theory Named
-  imports Type Variable "../00Utils/Utils"
+theory Typed
+  imports Type "../01Source/Variable" "../00Utils/Utils"
 begin
 
-datatype nexpr = 
-  NVar var
-  | NConst nat
-  | NLam var ty nexpr
-  | NApp nexpr nexpr
+datatype texpr = 
+  TVar var
+  | TConst nat
+  | TLam var ty texpr
+  | TApp texpr texpr
 
-primrec all_vars :: "nexpr \<Rightarrow> var set" where
-  "all_vars (NVar x) = {x}"
-| "all_vars (NConst k) = {}"
-| "all_vars (NLam x t e) = insert x (all_vars e)"
-| "all_vars (NApp e\<^sub>1 e\<^sub>2) = all_vars e\<^sub>1 \<union> all_vars e\<^sub>2"
+primrec all_vars :: "texpr \<Rightarrow> var set" where
+  "all_vars (TVar x) = {x}"
+| "all_vars (TConst k) = {}"
+| "all_vars (TLam x t e) = insert x (all_vars e)"
+| "all_vars (TApp e\<^sub>1 e\<^sub>2) = all_vars e\<^sub>1 \<union> all_vars e\<^sub>2"
 
-primrec binders :: "nexpr \<Rightarrow> var set" where
-  "binders (NVar x) = {}"
-| "binders (NConst k) = {}"
-| "binders (NLam x t e) = insert x (binders e)"
-| "binders (NApp e\<^sub>1 e\<^sub>2) = binders e\<^sub>1 \<union> binders e\<^sub>2"
+primrec binders :: "texpr \<Rightarrow> var set" where
+  "binders (TVar x) = {}"
+| "binders (TConst k) = {}"
+| "binders (TLam x t e) = insert x (binders e)"
+| "binders (TApp e\<^sub>1 e\<^sub>2) = binders e\<^sub>1 \<union> binders e\<^sub>2"
 
-primrec free_vars :: "nexpr \<Rightarrow> var set" where
-  "free_vars (NVar x) = {x}"
-| "free_vars (NConst k) = {}"
-| "free_vars (NLam x t e) = free_vars e - {x}"
-| "free_vars (NApp e\<^sub>1 e\<^sub>2) = free_vars e\<^sub>1 \<union> free_vars e\<^sub>2"
+primrec free_vars :: "texpr \<Rightarrow> var set" where
+  "free_vars (TVar x) = {x}"
+| "free_vars (TConst k) = {}"
+| "free_vars (TLam x t e) = free_vars e - {x}"
+| "free_vars (TApp e\<^sub>1 e\<^sub>2) = free_vars e\<^sub>1 \<union> free_vars e\<^sub>2"
 
-inductive typecheckn :: "(var \<rightharpoonup> ty) \<Rightarrow> nexpr \<Rightarrow> ty \<Rightarrow> bool" (infix "\<turnstile>\<^sub>n _ :" 50) where
-  tcn_var [simp]: "\<Gamma> x = Some t \<Longrightarrow> \<Gamma> \<turnstile>\<^sub>n NVar x : t"
-| tcn_const [simp]: "\<Gamma> \<turnstile>\<^sub>n NConst k : Base"
-| tcn_lam [simp]: "\<Gamma>(x \<mapsto> t\<^sub>1) \<turnstile>\<^sub>n e : t\<^sub>2 \<Longrightarrow> \<Gamma> \<turnstile>\<^sub>n NLam x t\<^sub>1 e : Arrow t\<^sub>1 t\<^sub>2"
-| tcn_app [simp]: "\<Gamma> \<turnstile>\<^sub>n e\<^sub>1 : Arrow t\<^sub>1 t\<^sub>2 \<Longrightarrow> \<Gamma> \<turnstile>\<^sub>n e\<^sub>2 : t\<^sub>1 \<Longrightarrow> \<Gamma> \<turnstile>\<^sub>n NApp e\<^sub>1 e\<^sub>2 : t\<^sub>2"
+inductive typecheckn :: "(var \<rightharpoonup> ty) \<Rightarrow> texpr \<Rightarrow> ty \<Rightarrow> bool" (infix "\<turnstile>\<^sub>n _ :" 50) where
+  tcn_var [simp]: "\<Gamma> x = Some t \<Longrightarrow> \<Gamma> \<turnstile>\<^sub>n TVar x : t"
+| tcn_const [simp]: "\<Gamma> \<turnstile>\<^sub>n TConst k : Base"
+| tcn_lam [simp]: "\<Gamma>(x \<mapsto> t\<^sub>1) \<turnstile>\<^sub>n e : t\<^sub>2 \<Longrightarrow> \<Gamma> \<turnstile>\<^sub>n TLam x t\<^sub>1 e : Arrow t\<^sub>1 t\<^sub>2"
+| tcn_app [simp]: "\<Gamma> \<turnstile>\<^sub>n e\<^sub>1 : Arrow t\<^sub>1 t\<^sub>2 \<Longrightarrow> \<Gamma> \<turnstile>\<^sub>n e\<^sub>2 : t\<^sub>1 \<Longrightarrow> \<Gamma> \<turnstile>\<^sub>n TApp e\<^sub>1 e\<^sub>2 : t\<^sub>2"
 
-inductive_cases [elim]: "\<Gamma> \<turnstile>\<^sub>n NVar x : t"
-inductive_cases [elim]: "\<Gamma> \<turnstile>\<^sub>n NConst k : t"
-inductive_cases [elim]: "\<Gamma> \<turnstile>\<^sub>n NLam x t' e : t"
-inductive_cases [elim]: "\<Gamma> \<turnstile>\<^sub>n NApp e\<^sub>1 e\<^sub>2 : t"
+inductive_cases [elim]: "\<Gamma> \<turnstile>\<^sub>n TVar x : t"
+inductive_cases [elim]: "\<Gamma> \<turnstile>\<^sub>n TConst k : t"
+inductive_cases [elim]: "\<Gamma> \<turnstile>\<^sub>n TLam x t' e : t"
+inductive_cases [elim]: "\<Gamma> \<turnstile>\<^sub>n TApp e\<^sub>1 e\<^sub>2 : t"
 
-primrec valn :: "nexpr \<Rightarrow> bool" where
-  "valn (NVar x) = False"
-| "valn (NConst k) = True" 
-| "valn (NLam x t e) = True" 
-| "valn (NApp e\<^sub>1 e\<^sub>2) = False" 
+primrec valn :: "texpr \<Rightarrow> bool" where
+  "valn (TVar x) = False"
+| "valn (TConst k) = True" 
+| "valn (TLam x t e) = True" 
+| "valn (TApp e\<^sub>1 e\<^sub>2) = False" 
 
-primrec subst_var :: "var \<Rightarrow> var \<Rightarrow> nexpr \<Rightarrow> nexpr" where
-  "subst_var x x' (NVar y) = NVar (if x = y then x' else y)"
-| "subst_var x x' (NConst k) = NConst k"
-| "subst_var x x' (NLam y t e) = NLam y t (if x = y then e else subst_var x x' e)"
-| "subst_var x x' (NApp e\<^sub>1 e\<^sub>2) = NApp (subst_var x x' e\<^sub>1) (subst_var x x' e\<^sub>2)"
+primrec subst_var :: "var \<Rightarrow> var \<Rightarrow> texpr \<Rightarrow> texpr" where
+  "subst_var x x' (TVar y) = TVar (if x = y then x' else y)"
+| "subst_var x x' (TConst k) = TConst k"
+| "subst_var x x' (TLam y t e) = TLam y t (if x = y then e else subst_var x x' e)"
+| "subst_var x x' (TApp e\<^sub>1 e\<^sub>2) = TApp (subst_var x x' e\<^sub>1) (subst_var x x' e\<^sub>2)"
 
 lemma [simp]: "size (subst_var x x' e) = size e"
   by (induction e) simp_all
 
-fun substn :: "var \<Rightarrow> nexpr \<Rightarrow> nexpr \<Rightarrow> nexpr" where
-  "substn x e' (NVar y) = (if x = y then e' else NVar y)"
-| "substn x e' (NConst k) = NConst k"
-| "substn x e' (NLam y t e) = (
+fun substn :: "var \<Rightarrow> texpr \<Rightarrow> texpr \<Rightarrow> texpr" where
+  "substn x e' (TVar y) = (if x = y then e' else TVar y)"
+| "substn x e' (TConst k) = TConst k"
+| "substn x e' (TLam y t e) = (
     let z = fresh (all_vars e' \<union> all_vars e \<union> {x, y})
-    in NLam z t (substn x e' (subst_var y z e)))"
-| "substn x e' (NApp e\<^sub>1 e\<^sub>2) = NApp (substn x e' e\<^sub>1) (substn x e' e\<^sub>2)"
+    in TLam z t (substn x e' (subst_var y z e)))"
+| "substn x e' (TApp e\<^sub>1 e\<^sub>2) = TApp (substn x e' e\<^sub>1) (substn x e' e\<^sub>2)"
 
-inductive evaln :: "nexpr \<Rightarrow> nexpr \<Rightarrow> bool" (infix "\<Down>" 50) where
-  evn_const [simp]: "NConst k \<Down> NConst k"
-| evn_lam [simp]: "NLam x t e \<Down> NLam x t e"
-| evn_app [simp]: "e\<^sub>1 \<Down> NLam x t e\<^sub>1' \<Longrightarrow> e\<^sub>2 \<Down> v\<^sub>2 \<Longrightarrow> substn x v\<^sub>2 e\<^sub>1' \<Down> v \<Longrightarrow> NApp e\<^sub>1 e\<^sub>2 \<Down> v"
+inductive evaln :: "texpr \<Rightarrow> texpr \<Rightarrow> bool" (infix "\<Down>" 50) where
+  evn_const [simp]: "TConst k \<Down> TConst k"
+| evn_lam [simp]: "TLam x t e \<Down> TLam x t e"
+| evn_app [simp]: "e\<^sub>1 \<Down> TLam x t e\<^sub>1' \<Longrightarrow> e\<^sub>2 \<Down> v\<^sub>2 \<Longrightarrow> substn x v\<^sub>2 e\<^sub>1' \<Down> v \<Longrightarrow> TApp e\<^sub>1 e\<^sub>2 \<Down> v"
 
 lemma [simp]: "finite (all_vars e)"
   by (induction e) simp_all
 
 lemma [simp]: "free_vars e \<subseteq> insert x xs \<Longrightarrow> free_vars (subst_var x x' e) \<subseteq> insert x' xs"
 proof (induction e arbitrary: xs)
-  case (NLam y t e)
+  case (TLam y t e)
   hence "free_vars e \<subseteq> insert x (insert y xs)" by auto
-  with NLam have "free_vars (subst_var x x' e) \<subseteq> insert x' (insert y xs)" by simp
-  with NLam show ?case by auto
+  with TLam have "free_vars (subst_var x x' e) \<subseteq> insert x' (insert y xs)" by simp
+  with TLam show ?case by auto
 qed auto
 
 lemma free_vars_subst [simp]: "free_vars e \<subseteq> insert x xs \<Longrightarrow> free_vars e' \<subseteq> xs \<Longrightarrow> 
@@ -101,11 +101,11 @@ lemma free_vars_subs [simp]: "\<Gamma> \<turnstile>\<^sub>n e : t \<Longrightarr
 lemma [simp]: "Map.empty \<turnstile>\<^sub>n e : t \<Longrightarrow> free_vars e = {}"
   using free_vars_subs by fastforce
 
-lemma canonical_basen [dest]: "\<Gamma> \<turnstile>\<^sub>n e : Base \<Longrightarrow> valn e \<Longrightarrow> \<exists>k. e = NConst k"
+lemma canonical_basen [dest]: "\<Gamma> \<turnstile>\<^sub>n e : Base \<Longrightarrow> valn e \<Longrightarrow> \<exists>k. e = TConst k"
   by (induction \<Gamma> e Base rule: typecheckn.induct) simp_all
 
 lemma canonical_arrown [dest]: "\<Gamma> \<turnstile>\<^sub>n e : Arrow t\<^sub>1 t\<^sub>2 \<Longrightarrow> valn e \<Longrightarrow> 
-    \<exists>x e'. e = NLam x t\<^sub>1 e' \<and> \<Gamma>(x \<mapsto> t\<^sub>1) \<turnstile>\<^sub>n e' : t\<^sub>2"
+    \<exists>x e'. e = TLam x t\<^sub>1 e' \<and> \<Gamma>(x \<mapsto> t\<^sub>1) \<turnstile>\<^sub>n e' : t\<^sub>2"
   by (induction \<Gamma> e "Arrow t\<^sub>1 t\<^sub>2" rule: typecheckn.induct) simp_all
 
 (* Progress not directly provable here, due to lack of proof of termination.
@@ -153,14 +153,14 @@ lemma val_no_evaln: "e \<Down> v \<Longrightarrow> valn e \<Longrightarrow> v = 
 theorem determinismn: "e \<Down> v \<Longrightarrow> e \<Down> v' \<Longrightarrow> v = v'"
 proof (induction e v arbitrary: v' rule: evaln.induct)
   case (evn_const k)
-  thus ?case by (induction "NConst k" v' rule: evaln.induct) simp_all
+  thus ?case by (induction "TConst k" v' rule: evaln.induct) simp_all
 next
   case (evn_lam x t e)
-  thus ?case by (induction "NLam x t e" v' rule: evaln.induct) simp_all
+  thus ?case by (induction "TLam x t e" v' rule: evaln.induct) simp_all
 next
   case (evn_app e\<^sub>1 x t e\<^sub>1' e\<^sub>2 v\<^sub>2 v)
   from evn_app(7, 1, 2, 3, 4, 5, 6) show ?case 
-    by (induction "NApp e\<^sub>1 e\<^sub>2" v' rule: evaln.induct) blast+
+    by (induction "TApp e\<^sub>1 e\<^sub>2" v' rule: evaln.induct) blast+
 qed
 
 end
