03Debruijn/NameRemoval.thy
@@ -1,14 +1,14 @@
 theory NameRemoval
-  imports "../02Source/Named" BigStep "../00Utils/AssocList"
+  imports "../02Typed/Typed" BigStep "../00Utils/AssocList"
 begin
 
-fun convert' :: "var list \<Rightarrow> nexpr \<Rightarrow> dexpr" where
-  "convert' \<Phi> (NVar x) = DVar (the (idx_of \<Phi> x))"
-| "convert' \<Phi> (NConst k) = DConst k"
-| "convert' \<Phi> (NLam x t e) = DLam t (convert' (insert_at 0 x \<Phi>) e)"
-| "convert' \<Phi> (NApp e\<^sub>1 e\<^sub>2) = DApp (convert' \<Phi> e\<^sub>1) (convert' \<Phi> e\<^sub>2)"
+fun convert' :: "var list \<Rightarrow> texpr \<Rightarrow> dexpr" where
+  "convert' \<Phi> (TVar x) = DVar (the (idx_of \<Phi> x))"
+| "convert' \<Phi> (TConst k) = DConst k"
+| "convert' \<Phi> (TLam x t e) = DLam t (convert' (insert_at 0 x \<Phi>) e)"
+| "convert' \<Phi> (TApp e\<^sub>1 e\<^sub>2) = DApp (convert' \<Phi> e\<^sub>1) (convert' \<Phi> e\<^sub>2)"
 
-definition convert :: "nexpr \<Rightarrow> dexpr" where
+definition convert :: "texpr \<Rightarrow> dexpr" where
   "convert e = convert' [] e"
 
 lemma [simp]: "map_of \<Gamma> \<turnstile>\<^sub>n e : t \<Longrightarrow> mset (map fst \<Gamma>) = mset \<Phi> \<Longrightarrow> 
@@ -39,11 +39,11 @@ lemma [simp]: "valn e \<Longrightarrow> vald (convert' \<Phi> e)"
 lemma [simp]: "y \<notin> all_vars e \<Longrightarrow> x \<le> length \<Phi> \<Longrightarrow> free_vars e \<subseteq> set \<Phi> \<Longrightarrow>
   convert' (insert_at x y \<Phi>) e = incrd x (convert' \<Phi> e)"
 proof (induction e arbitrary: x \<Phi>)
-  case (NVar z)
+  case (TVar z)
   moreover then obtain w where "idx_of \<Phi> z = Some w" by fastforce
   ultimately show ?case by simp
 next
-  case (NLam z t e)
+  case (TLam z t e)
   moreover hence "free_vars e \<subseteq> set (insert_at 0 z \<Phi>)" by auto
   ultimately show ?case by simp
 qed simp_all
@@ -56,14 +56,14 @@ lemma [simp]: "y \<le> length \<Phi> \<Longrightarrow> y precedes x in \<Phi> \<
   free_vars e \<subseteq> insert x (set \<Phi>) \<Longrightarrow> 
     convert' (insert_at y x' \<Phi>) (subst_var x x' e) = convert' (insert_at y x \<Phi>) e"
 proof (induction e arbitrary: y \<Phi>)
-  case (NLam z t e)
+  case (TLam z t e)
   thus ?case
   proof (cases "x = z")
     case False
-    with NLam have X: "Suc y precedes x in insert_at 0 z \<Phi>" by (simp split: option.splits) 
-    from NLam have Y: "Suc y precedes x' in insert_at 0 z \<Phi>" by (simp split: option.splits) 
-    from NLam have "free_vars e \<subseteq> insert x (set (insert_at 0 z \<Phi>))" by auto
-    with NLam False X Y show ?thesis by simp
+    with TLam have X: "Suc y precedes x in insert_at 0 z \<Phi>" by (simp split: option.splits) 
+    from TLam have Y: "Suc y precedes x' in insert_at 0 z \<Phi>" by (simp split: option.splits) 
+    from TLam have "free_vars e \<subseteq> insert x (set (insert_at 0 z \<Phi>))" by auto
+    with TLam False X Y show ?thesis by simp
   qed (simp_all split: option.splits)
 qed (auto split: option.splits)
 
@@ -99,9 +99,9 @@ qed simp_all
 theorem correctnd [simp]: "e \<Down> v \<Longrightarrow> free_vars e = {} \<Longrightarrow> convert e \<Down>\<^sub>d convert v"
 proof (induction e v rule: evaln.induct)
   case (evn_app e\<^sub>1 x t e\<^sub>1' e\<^sub>2 v\<^sub>2 v)
-  hence "e\<^sub>1 \<Down> NLam x t e\<^sub>1'" by simp
+  hence "e\<^sub>1 \<Down> TLam x t e\<^sub>1'" by simp
   moreover from evn_app have "free_vars e\<^sub>1 = {}" by simp
-  ultimately have "free_vars (NLam x t e\<^sub>1') = {}" by (metis free_vars_eval)
+  ultimately have "free_vars (TLam x t e\<^sub>1') = {}" by (metis free_vars_eval)
   hence X: "free_vars e\<^sub>1' \<subseteq> insert x (set [])" by simp
   moreover from evn_app have Y: "free_vars v\<^sub>2 \<subseteq> set []" by simp
   ultimately have "free_vars (substn x v\<^sub>2 e\<^sub>1') \<subseteq> set []" by (metis free_vars_subst)
@@ -115,35 +115,35 @@ lemma convert_val_back: "vald (convert e) \<Longrightarrow> valn e"
   by (simp add: convert_def)
 
 lemma [dest]: "DApp e\<^sub>d\<^sub>1 e\<^sub>d\<^sub>2 = convert e\<^sub>n \<Longrightarrow> 
-    \<exists>e\<^sub>n\<^sub>1 e\<^sub>n\<^sub>2. e\<^sub>n = NApp e\<^sub>n\<^sub>1 e\<^sub>n\<^sub>2 \<and> e\<^sub>d\<^sub>1 = convert e\<^sub>n\<^sub>1 \<and> e\<^sub>d\<^sub>2 = convert e\<^sub>n\<^sub>2"
+    \<exists>e\<^sub>n\<^sub>1 e\<^sub>n\<^sub>2. e\<^sub>n = TApp e\<^sub>n\<^sub>1 e\<^sub>n\<^sub>2 \<and> e\<^sub>d\<^sub>1 = convert e\<^sub>n\<^sub>1 \<and> e\<^sub>d\<^sub>2 = convert e\<^sub>n\<^sub>2"
   by (cases e\<^sub>n) (simp_all add: convert_def)
 
 lemma [dest]: "DLam t e\<^sub>d = convert e\<^sub>n \<Longrightarrow> 
-    \<exists>x e\<^sub>n'. e\<^sub>n = NLam x t e\<^sub>n' \<and> e\<^sub>d = convert' [x] e\<^sub>n'"
+    \<exists>x e\<^sub>n'. e\<^sub>n = TLam x t e\<^sub>n' \<and> e\<^sub>d = convert' [x] e\<^sub>n'"
   by (cases e\<^sub>n) (simp_all add: convert_def)
 
 theorem completend [simp]: "convert e\<^sub>n \<Down>\<^sub>d v\<^sub>d \<Longrightarrow> free_vars e\<^sub>n = {} \<Longrightarrow> 
   \<exists>v\<^sub>n. e\<^sub>n \<Down> v\<^sub>n \<and> v\<^sub>d = convert v\<^sub>n"
 proof (induction "convert e\<^sub>n" v\<^sub>d arbitrary: e\<^sub>n rule: big_evald.induct)
   case (bevd_const k)
-  hence "e\<^sub>n \<Down> NConst k \<and> DConst k = convert (NConst k)" by (cases e\<^sub>n) (simp_all add: convert_def)
+  hence "e\<^sub>n \<Down> TConst k \<and> DConst k = convert (TConst k)" by (cases e\<^sub>n) (simp_all add: convert_def)
   thus ?case by fastforce
 next
   case (bevd_lam t e)
-  then obtain x e' where "e\<^sub>n = NLam x t e' \<and> e = convert' [x] e'" 
+  then obtain x e' where "e\<^sub>n = TLam x t e' \<and> e = convert' [x] e'" 
     by (cases e\<^sub>n) (simp_all add: convert_def)
-  hence "e\<^sub>n \<Down> NLam x t e' \<and> DLam t e = convert (NLam x t e')" by (simp add: convert_def)
+  hence "e\<^sub>n \<Down> TLam x t e' \<and> DLam t e = convert (TLam x t e')" by (simp add: convert_def)
   thus ?case by fastforce
 next
   case (bevd_app e\<^sub>1 t e\<^sub>1' e\<^sub>2 v\<^sub>2 v)
-  then obtain e\<^sub>n\<^sub>1 e\<^sub>n\<^sub>2 where E: "e\<^sub>n = NApp e\<^sub>n\<^sub>1 e\<^sub>n\<^sub>2 \<and> e\<^sub>1 = convert e\<^sub>n\<^sub>1 \<and> e\<^sub>2 = convert e\<^sub>n\<^sub>2" 
+  then obtain e\<^sub>n\<^sub>1 e\<^sub>n\<^sub>2 where E: "e\<^sub>n = TApp e\<^sub>n\<^sub>1 e\<^sub>n\<^sub>2 \<and> e\<^sub>1 = convert e\<^sub>n\<^sub>1 \<and> e\<^sub>2 = convert e\<^sub>n\<^sub>2" 
     by (cases e\<^sub>n) (simp_all add: convert_def)
   with bevd_app obtain v\<^sub>n\<^sub>1 where V1: "e\<^sub>n\<^sub>1 \<Down> v\<^sub>n\<^sub>1 \<and> DLam t e\<^sub>1' = convert v\<^sub>n\<^sub>1" by fastforce
-  then obtain x e\<^sub>n\<^sub>1' where X: "v\<^sub>n\<^sub>1 = NLam x t e\<^sub>n\<^sub>1' \<and> e\<^sub>1' = convert' [x] e\<^sub>n\<^sub>1'"
+  then obtain x e\<^sub>n\<^sub>1' where X: "v\<^sub>n\<^sub>1 = TLam x t e\<^sub>n\<^sub>1' \<and> e\<^sub>1' = convert' [x] e\<^sub>n\<^sub>1'"
     by (cases v\<^sub>n\<^sub>1) (simp_all add: convert_def)
   from bevd_app E obtain v\<^sub>n\<^sub>2 where V2: "e\<^sub>n\<^sub>2 \<Down> v\<^sub>n\<^sub>2 \<and> v\<^sub>2 = convert v\<^sub>n\<^sub>2" by fastforce
   from bevd_app E have "free_vars e\<^sub>n\<^sub>1 = {}" by simp
-  with V1 X have "free_vars (NLam x t e\<^sub>n\<^sub>1') = {}" by (metis free_vars_eval)
+  with V1 X have "free_vars (TLam x t e\<^sub>n\<^sub>1') = {}" by (metis free_vars_eval)
   hence Y: "free_vars e\<^sub>n\<^sub>1' \<subseteq> {x}" by simp
   from bevd_app E have "free_vars e\<^sub>n\<^sub>2 = {}" by simp
   with V2 have Z: "free_vars v\<^sub>n\<^sub>2 = {}" by auto
@@ -151,7 +151,7 @@ next
   with bevd_app X V2 Y Z have "\<exists>v\<^sub>n. substn x v\<^sub>n\<^sub>2 e\<^sub>n\<^sub>1' \<Down> v\<^sub>n \<and> v = convert v\<^sub>n" 
     by (simp add: convert_def)
   then obtain v\<^sub>n where "substn x v\<^sub>n\<^sub>2 e\<^sub>n\<^sub>1' \<Down> v\<^sub>n \<and> v = convert v\<^sub>n" by fastforce
-  with V1 X V2 have "NApp e\<^sub>n\<^sub>1 e\<^sub>n\<^sub>2 \<Down> v\<^sub>n \<and> v = convert v\<^sub>n" by fastforce
+  with V1 X V2 have "TApp e\<^sub>n\<^sub>1 e\<^sub>n\<^sub>2 \<Down> v\<^sub>n \<and> v = convert v\<^sub>n" by fastforce
   with E show ?case by fastforce
 qed
 
