Compiler.thy
@@ -1,20 +1,19 @@
 theory Compiler
-  imports "02Source/AlgorithmicTypechecking" Printing "04Stack/StackConversion" 
-          "12UnstructuredMemory/Unstructuring" 
+  imports Printing "04Stack/StackConversion" "12UnstructuredMemory/Unstructuring" 
 begin
 
-abbreviation compile :: "nexpr \<Rightarrow> byte_code list" where 
+abbreviation compile :: "texpr \<Rightarrow> byte_code list" where 
   "compile \<equiv> flatten_code \<circ> tco \<circ> encode \<circ> convert"
 
 lemma [simp]: "live_frame (env, tco_cd (encode e), tco_r (encode e))"
   by (induction e) simp_all
 
-theorem tc_terminationn: "typechecks e \<Longrightarrow> compile e = cd \<Longrightarrow> 
+theorem tc_terminationn: "\<exists>t. Map.empty \<turnstile>\<^sub>n e : t \<Longrightarrow> compile e = cd \<Longrightarrow> 
   \<exists>v. valn v \<and> e \<Down> v \<and> 
     (\<exists>h hp e ep v\<^sub>u s. iter (\<leadsto>\<^sub>u) (US nmem 0 0 0 nmem 0 nmem 0 (nmem(0 := 0)) 1 (length cd) cd) 
-      (US h hp 0 0 e ep v\<^sub>u 1 s 0 0 cd) \<and> print_uclosure h (v\<^sub>u 0) = print_nexpr v)"
+      (US h hp 0 0 e ep v\<^sub>u 1 s 0 0 cd) \<and> print_uclosure h (v\<^sub>u 0) = print_texpr v)"
 proof -
-  assume "typechecks e"
+  assume "\<exists>t. Map.empty \<turnstile>\<^sub>n e : t"
   then obtain t where TN: "Map.empty \<turnstile>\<^sub>n e : t" by fastforce
   then obtain v\<^sub>n where EN: "e \<Down> v\<^sub>n" by fastforce
   hence VN: "valn v\<^sub>n" by simp
@@ -28,7 +27,7 @@ proof -
     by (metis tcc_state_ev tcc_nil tcc_snil tcc_scons_ret latest_environment.simps(4))
   with ES VD EN obtain c where EC: "iter (\<leadsto>\<^sub>c) (CSE [CReturn []] [] (convert e)) (CSC [] c) \<and> 
     declosure c = convert v\<^sub>n" by fastforce
-  with VN have VC: "print_closure c = print_nexpr v\<^sub>n" by simp
+  with VN have VC: "print_closure c = print_texpr v\<^sub>n" by simp
   from TC EC have "iter (\<leadsto>\<^sub>t) (encode_state (CSE [CReturn []] [] (convert e))) 
     (encode_state (CSC [] c))" by (metis iter_completet)
   hence "iter (\<leadsto>\<^sub>t) (TS [] [([], encode (convert e))]) (TS [encode_closure c] [])" 
@@ -47,12 +46,12 @@ proof -
       tco_val (encode_closure c) = unflatten_closure cd v\<^sub>b" 
     by (metis evalb_end byte_code_state.sel(3))
   hence "print_bclosure v\<^sub>b = print_tco_closure (tco_val (encode_closure c))" by simp
-  with VC have VB: "print_bclosure v\<^sub>b = print_nexpr v\<^sub>n" by simp
+  with VC have VB: "print_bclosure v\<^sub>b = print_texpr v\<^sub>n" by simp
   from EB obtain \<Sigma>\<^sub>h' where EH: "iter (\<leadsto>\<^sub>h) (HS hempty [] [([], length cd)] cd) \<Sigma>\<^sub>h' \<and> 
     BS [v\<^sub>b] [] cd = unheap \<Sigma>\<^sub>h'" by fastforce
   then obtain h\<^sub>h v\<^sub>h where SH: "\<Sigma>\<^sub>h' = HS h\<^sub>h [v\<^sub>h] [] cd \<and> v\<^sub>b = unheap_closure h\<^sub>h v\<^sub>h" 
     using unheap_empty by blast
-  with VB have VH: "print_hclosure (hlookup h\<^sub>h v\<^sub>h) = print_nexpr v\<^sub>n" by simp
+  with VB have VH: "print_hclosure (hlookup h\<^sub>h v\<^sub>h) = print_texpr v\<^sub>n" by simp
   have HS: "heap_structured (HS hempty [] [([], length cd)] cd)" by simp
   have CES: "unchain_state (CES hempty hempty [] [(0, length cd)] cd) = 
     HS hempty [] [([], length cd)] cd" by simp
@@ -60,12 +59,12 @@ proof -
     HS h\<^sub>h [v\<^sub>h] [] cd = unchain_state \<Sigma>\<^sub>c\<^sub>e'" by fastforce
   then obtain h\<^sub>c\<^sub>e env\<^sub>h where VCE: "\<Sigma>\<^sub>c\<^sub>e' = CES h\<^sub>c\<^sub>e env\<^sub>h [v\<^sub>h] [] cd \<and> h\<^sub>h = unchain_heap h\<^sub>c\<^sub>e env\<^sub>h" 
     by (metis unchain_state_reverse map_is_Nil_conv)
-  with VH have PCE: "print_ceclosure (hlookup h\<^sub>c\<^sub>e v\<^sub>h) = print_nexpr v\<^sub>n" by (metis print_ce)
+  with VH have PCE: "print_ceclosure (hlookup h\<^sub>c\<^sub>e v\<^sub>h) = print_texpr v\<^sub>n" by (metis print_ce)
   from ECE VCE have "iter (\<leadsto>\<^sub>f) (flatten (CES hempty hempty [] [(0, length cd)] cd))
     (flatten (CES h\<^sub>c\<^sub>e env\<^sub>h [v\<^sub>h] [] cd))" by (metis completef_iter)
   hence EF: "iter (\<leadsto>\<^sub>f) (FS (H nmem 0) (H nmem 0) [] [length cd, 0] cd)
      (FS (flatten_values h\<^sub>c\<^sub>e) (flatten_environment env\<^sub>h) [v\<^sub>h] [] cd)" by (simp add: hempty_def)
-  from PCE have PF: "print_ceclosure (get_closure (flatten_values h\<^sub>c\<^sub>e) v\<^sub>h) = print_nexpr v\<^sub>n" 
+  from PCE have PF: "print_ceclosure (get_closure (flatten_values h\<^sub>c\<^sub>e) v\<^sub>h) = print_texpr v\<^sub>n" 
     by (simp del: get_closure.simps)
   from C have "cd \<noteq> []" by auto
   with EF have "\<exists>\<Sigma>\<^sub>u'. iter (\<leadsto>\<^sub>u) (US nmem 0 0 0 nmem 0 nmem 0 (nmem(0 := 0)) 1 (length cd) cd) \<Sigma>\<^sub>u' \<and> 
@@ -86,7 +85,7 @@ proof -
 
 
 
-  from PF VU VSU have PU: "print_uclosure h\<^sub>u (vs\<^sub>u 0) = print_nexpr v\<^sub>n" by (metis print_u)
+  from PF VU VSU have PU: "print_uclosure h\<^sub>u (vs\<^sub>u 0) = print_texpr v\<^sub>n" by (metis print_u)
 
 
 
