01Source/Named.thy
@@ -1,0 +1,108 @@
+theory Named
+  imports Variable "../00Utils/Utils"
+begin
+
+datatype nexpr = 
+  NVar var
+  | NConst nat
+  | NLam var nexpr
+  | NApp nexpr nexpr
+
+primrec all_vars :: "nexpr \<Rightarrow> var set" where
+  "all_vars (NVar x) = {x}"
+| "all_vars (NConst k) = {}"
+| "all_vars (NLam x e) = insert x (all_vars e)"
+| "all_vars (NApp e\<^sub>1 e\<^sub>2) = all_vars e\<^sub>1 \<union> all_vars e\<^sub>2"
+
+primrec binders :: "nexpr \<Rightarrow> var set" where
+  "binders (NVar x) = {}"
+| "binders (NConst k) = {}"
+| "binders (NLam x e) = insert x (binders e)"
+| "binders (NApp e\<^sub>1 e\<^sub>2) = binders e\<^sub>1 \<union> binders e\<^sub>2"
+
+primrec free_vars :: "nexpr \<Rightarrow> var set" where
+  "free_vars (NVar x) = {x}"
+| "free_vars (NConst k) = {}"
+| "free_vars (NLam x e) = free_vars e - {x}"
+| "free_vars (NApp e\<^sub>1 e\<^sub>2) = free_vars e\<^sub>1 \<union> free_vars e\<^sub>2"
+
+primrec valn :: "nexpr \<Rightarrow> bool" where
+  "valn (NVar x) = False"
+| "valn (NConst k) = True" 
+| "valn (NLam x e) = True" 
+| "valn (NApp e\<^sub>1 e\<^sub>2) = False" 
+
+primrec subst_var :: "var \<Rightarrow> var \<Rightarrow> nexpr \<Rightarrow> nexpr" where
+  "subst_var x x' (NVar y) = NVar (if x = y then x' else y)"
+| "subst_var x x' (NConst k) = NConst k"
+| "subst_var x x' (NLam y e) = NLam y (if x = y then e else subst_var x x' e)"
+| "subst_var x x' (NApp e\<^sub>1 e\<^sub>2) = NApp (subst_var x x' e\<^sub>1) (subst_var x x' e\<^sub>2)"
+
+lemma [simp]: "size (subst_var x x' e) = size e"
+  by (induction e) simp_all
+
+fun substn :: "var \<Rightarrow> nexpr \<Rightarrow> nexpr \<Rightarrow> nexpr" where
+  "substn x e' (NVar y) = (if x = y then e' else NVar y)"
+| "substn x e' (NConst k) = NConst k"
+| "substn x e' (NLam y e) = (
+    let z = fresh (all_vars e' \<union> all_vars e \<union> {x, y})
+    in NLam z (substn x e' (subst_var y z e)))"
+| "substn x e' (NApp e\<^sub>1 e\<^sub>2) = NApp (substn x e' e\<^sub>1) (substn x e' e\<^sub>2)"
+
+inductive evaln :: "nexpr \<Rightarrow> nexpr \<Rightarrow> bool" (infix "\<Down>" 50) where
+  evn_const [simp]: "NConst k \<Down> NConst k"
+| evn_lam [simp]: "NLam x e \<Down> NLam x e"
+| evn_app [simp]: "e\<^sub>1 \<Down> NLam x e\<^sub>1' \<Longrightarrow> e\<^sub>2 \<Down> v\<^sub>2 \<Longrightarrow> substn x v\<^sub>2 e\<^sub>1' \<Down> v \<Longrightarrow> NApp e\<^sub>1 e\<^sub>2 \<Down> v"
+
+lemma [simp]: "finite (all_vars e)"
+  by (induction e) simp_all
+
+lemma [simp]: "free_vars e \<subseteq> insert x xs \<Longrightarrow> free_vars (subst_var x x' e) \<subseteq> insert x' xs"
+proof (induction e arbitrary: xs)
+  case (NLam y e)
+  hence "free_vars e \<subseteq> insert x (insert y xs)" by auto
+  with NLam have "free_vars (subst_var x x' e) \<subseteq> insert x' (insert y xs)" by simp
+  with NLam show ?case by auto
+qed auto
+
+lemma free_vars_subst [simp]: "free_vars e \<subseteq> insert x xs \<Longrightarrow> free_vars e' \<subseteq> xs \<Longrightarrow> 
+  free_vars (substn x e' e) \<subseteq> xs"
+proof (induction x e' e arbitrary: xs rule: substn.induct)
+  case (3 x e' y e)
+  let ?z = "fresh (all_vars e' \<union> all_vars e \<union> {x, y})"
+  from 3 have "free_vars e \<subseteq> insert y (insert x xs)" by auto
+  hence "free_vars (subst_var y ?z e) \<subseteq> insert ?z (insert x xs)" by simp
+  hence "free_vars (subst_var y ?z e) \<subseteq> insert x (insert ?z xs)" by auto
+  with 3 show ?case by (auto simp add: Let_def)
+qed auto
+
+lemma free_vars_eval [simp]: "e \<Down> v \<Longrightarrow> free_vars e = {} \<Longrightarrow> free_vars v = {}"
+proof (induction e v rule: evaln.induct)
+  case (evn_app e\<^sub>1 x e\<^sub>1' e\<^sub>2 v\<^sub>2 v)
+  hence "free_vars e\<^sub>1' \<subseteq> insert x {} \<and> free_vars v\<^sub>2 \<subseteq> {}" by simp
+  hence "free_vars (substn x v\<^sub>2 e\<^sub>1') \<subseteq> {}" by (metis free_vars_subst)
+  with evn_app show ?case by simp
+qed simp_all
+
+(* We, obviously, do not have safety here yet. The relevant proofs are in 02/Named. *)
+
+lemma [simp]: "e \<Down> v \<Longrightarrow> valn v"
+  by (induction e v rule: evaln.induct) simp_all
+
+lemma val_no_evaln: "e \<Down> v \<Longrightarrow> valn e \<Longrightarrow> v = e"
+  by (induction e v rule: evaln.induct) simp_all
+
+theorem determinismn: "e \<Down> v \<Longrightarrow> e \<Down> v' \<Longrightarrow> v = v'"
+proof (induction e v arbitrary: v' rule: evaln.induct)
+  case (evn_const k)
+  thus ?case by (induction "NConst k" v' rule: evaln.induct) simp_all
+next
+  case (evn_lam x e)
+  thus ?case by (induction "NLam x e" v' rule: evaln.induct) simp_all
+next
+  case (evn_app e\<^sub>1 x e\<^sub>1' e\<^sub>2 v\<^sub>2 v)
+  from evn_app(7, 1, 2, 3, 4, 5, 6) show ?case 
+    by (induction "NApp e\<^sub>1 e\<^sub>2" v' rule: evaln.induct) blast+
+qed
+
+end
